\documentclass[MathsNotesBase.tex]{subfiles}


\date{\vspace{-6ex}}


\begin{document}
\chapter*{Integration Techniques}


\section*{High-level Strategy}
\begin{itemize}
  \item If the power of an expression in parentheses is low, we can multiply it out. Single terms - however high the powers are - can always be integrated. What prevents us from doing this with high powers is that the number of terms explodes.
  \item If the power of an expression in parentheses is high, we need to look for a substitution or simplification.
  \item If we can manipulate the integrand so that we achieve a multiplication by f'(x) for some f(x) in the integrand, then we can make a u-substitution of f(x).
  \item In particular, if we can achieve $\frac{f'(x)}{f(x)}$ then we can integrate to $\ln\rvert{x}\lvert$.
  \item If the integrand involves something that we can't integrate but can differentiate, then use integration by parts.
  \item If the integral includes a term that will be "reduced" by differentiation, then use integration by parts.
\end{itemize}



\section*{U-substitution}
\bigskip

  \subsection*{$\int{(x+3)(x - 1)^5}dx$:}
   
  \begin{align*}
      &= \int{(u+4)u^5}du && (u=x-1)\\
      &= \int{u^6+4u^5}du && \\[8pt]
      &= \frac{u^7}{7}+\frac{2}{3}u^6 + c && \\[8pt]
      &= \frac{(x-1)^7}{7} + \frac{2}{3}(x-1)^6 + c && \\[8pt]
      &= (x-1)^6\left(\frac{(x-1)}{7} + \frac{2}{3}\right) + c && \\[8pt]
      &= \frac{1}{7}(x-1)^6\left(x + \frac{11}{3}\right) + c
  \end{align*}
  
  \bigskip
  Can also be done using integration by parts:
  
  \begin{align*}
      &\int{(x+3)(x - 1)^5}dx && \\
      &= \frac{1}{6}(x+3)(x-1)^6 - \frac{1}{6}\int{(x-1)^6}dx + c && (uv - \int{u'v}dx)\\
      &= \frac{1}{6}(x-1)^6\left[(x+3) - \frac{1}{7}(x-1)\right] + c && \\[8pt]
      &= \frac{1}{6}(x-1)^6\left(\frac{6x}{7}+\frac{22}{7}\right) + c && \\[8pt]
      &= \frac{1}{7}(x-1)^6(x+\frac{11}{3}) + c
  \end{align*}
  
  \bigskip\bigskip\bigskip
  
  \subsection*{$\int{\frac{x+5}{2x+3}}dx$:}
   
  \begin{align*}
      &= \frac{1}{2}\int{\frac{u + 7}{2u}}du && (u = 2x + 3; x = \frac{u - 3}{2}; du = 2dx)\\
      &= \frac{1}{2}\int{\frac{u}{2}}du + \frac{1}{2}\int{\frac{7}{2u}}du && \\[8pt]
      &= \frac{u}{4}+\frac{7}{4}\ln\lvert{u}\rvert + c && \\[8pt]
      &= \frac{2x + 3}{4} + \frac{7}{4}\ln\lvert{2x + 3}\rvert + c && \\[8pt]
  \end{align*}
  
  
  \subsection*{$\int{\frac{x^2 + 4}{x + 2}}dx$:}
   
  \begin{align*}
      &= \int{\frac{(x + 2)^2 - 4x}{x + 2}}dx && \\
      &= \int{x + 2}\ dx - \int{\frac{4x}{x + 2}}dx && \\[8pt]
      &= \frac{x^2}{2} + 2x -  \int{\frac{4u - 8}{u}}du + c && (u = x + 2, x = u - 2)\\[8pt]
      &= \frac{x^2}{2} + 2x - \int{\frac{4u}{u}}du + \int{\frac{8}{u}}du + c && \\[8pt]
      &= \frac{x^2}{2} + 2x - 4x - 8 + 8\ln\rvert{x + 2}\rvert + c \\
      &= \frac{x^2}{2} - 2x - 8 + 8\ln\rvert{x + 2}\rvert + c
  \end{align*}
  
  
  \subsection*{$\int{\frac{(3 + \ln{x})^2(2 - \ln{x})}{4x}\ dx}$:}
   
  \begin{align*}
      &\text{slow way:}\\
      &= \int{\frac{(3 + u)^2(2 - u)}{4}\ du} &&(u = \ln{x},\ du = \frac{1}{x}\ dx) \\[8pt]
      &= \frac{1}{4}\int{(9 + 6u + u^2)(2 - u)\ du} && (\text{Note: can just multiply this} \\
      &&&\text{out because of the low power)} \\[8pt]
      &= \frac{1}{4}\int{18 + 12u + 2u^2 - 9u - 6u^2 - u^3\ du} && \\[8pt]
      &= \frac{1}{4}\int{-u^3 - 4u^2 + 3u + 18\ du} && \\[8pt]
      &= \frac{1}{4}\left(\frac{-u^4}{4} - \frac{4u^3}{3} + \frac{3u^2}{2} + 18u\right) && \\[8pt]
      &= -\frac{1}{4}\left(\frac{1}{4}(\ln{x})^4 - \frac{4}{3}(\ln{x})^3 + \frac{3}{2}(\ln{x})^2 + 18\ln{x}\right) + c && \\[8pt]
      &= -\frac{1}{16}(\ln{x})^4 - \frac{1}{3}(\ln{x})^3 + \frac{3}{8}(\ln{x})^2 + \frac{9}{2}\ln{x} + c && \\[8pt]
      &\text{faster way:}\\
      &= \int{\frac{u^2(5 - u)}{4}\ du} && (u = \ln{x},\ du = \frac{1}{x}\ dx)\\[8pt]
      &= \frac{1}{4}\int{5u^2 - u^3\ du}\\[8pt]
      &= \frac{1}{4}\left(\frac{5}{3}(3 + \ln{x})^3 - \frac{1}{4}(3 + \ln{x})^4\right) + c
  \end{align*}
  
  
  \subsection*{$\int_0^9{\sqrt{4 - \sqrt{x}}}\ dx$:}
   
  \begin{align*}
      &= -2\int_4^1{\sqrt{u}(4 - u)\ du} &&(u = 4 - \sqrt{x},\ du = -\frac{1}{2\sqrt{x}}\ dx) \\
      &= 2\int_1^4{4u^\frac{1}{2} - u^\frac{3}{2}\ du} && \\
      &= 2\left[\frac{8}{3}u^\frac{3}{2} - \frac{2}{5}u^\frac{5}{2}\right]_1^4 + c && \\[8pt]
      &= 2\left[
        \left(\frac{8}{3}4^\frac{3}{2} - \frac{2}{5}4^\frac{5}{2}\right) - 
        \left(\frac{8}{3} - \frac{2}{5}\right)
      \right]_1^4 + c && \\[8pt]
      &= 2\left(
        \frac{64}{3} - \frac{64}{5} - \frac{8}{3} + \frac{2}{5} 
      \right) + c && \\[8pt]
      &= 2\left(
        \frac{56}{3} - \frac{62}{5} 
      \right) + c && \\[8pt]
      &= \frac{188}{15} + c && \\[8pt]
      \text{Note: if the }&\text{substitution were }\sqrt{x} \\
      \text{then we wou}&\text{ldn't get rid of the radical as:} \\
      \int_0^9{\sqrt{4 - \sqrt{x}}\ dx} &= 2\int_0^3{\sqrt{4 - u}(u)\ du} &&(u = \sqrt{x}) \\
  \end{align*}
  
  
  \subsection*{$\int{\sin{3x}\cos{4x}\ dx}$:}
   
  \begin{align*}
      &= \frac{1}{4}\sin{3x}\sin{4x} - \frac{3}{4}\int{\cos{3x}\sin{4x}\ dx} \\
      &= \frac{1}{4}\sin{3x}\sin{4x} - \frac{3}{4}\left[-\frac{1}{4}\cos{3x}\cos{4x} - \frac{3}{4}\int{\sin{3x}\cos{4x}\ dx}\right] \\
      &= \frac{1}{4}\sin{3x}\sin{4x} + \frac{3}{16}\cos{3x}\cos{4x} + \frac{9}{16}\int{\sin{3x}\cos{4x}\ dx} \\
      \iff \frac{7}{16}\int{\sin{3x}\cos{4x}\ dx} &= \frac{1}{4}\sin{3x}\sin{4x} + \frac{3}{16}\cos{3x}\cos{4x} \\
      \iff \int{\sin{3x}\cos{4x}\ dx} &= \frac{4}{7}\sin{3x}\sin{4x} + \frac{3}{7}\cos{3x}\cos{4x} \\
  \end{align*}

  
\bigskip
\bigskip
\bigskip
\bigskip


\section*{Integration By Parts}
\bigskip

  \subsection*{Derivation}
  \begin{align*}
      &&\frac{d}{dx}(uv) &= \frac{du}{dx}v + u\frac{dv}{dx} &\\
      &\implies &uv &= \int{v\frac{du}{dx}}\ dx + \int{u\frac{dv}{dx}}\ dx  &(\text{integrating wrt. $x$})\\
      &\iff &uv &= \int{u}\ dv + \int{v}\ du &\\
      &\iff &\int{u}\ dv &= uv - \int{v}\ du &
  \end{align*}
  
    \subsubsection*{Usage}
    \begin{align*}
      \int{f(x)\frac{dg}{dx}}\ dx &= f(x)(g(x) + c) - \int{(g(x) + c)\frac{df}{dx}}\ dx \\
      &= f(x)g(x) + cf(x) - \int{g(x)\frac{df}{dx}}\ dx + c\int{\frac{df}{dx}}\ dx \\
      &= f(x)g(x) + cf(x) - \int{g(x)\frac{df}{dx}}\ dx + cf(x) \\
      &= f(x)g(x) - \int{g(x)\frac{df}{dx}}\ dx \\
    \end{align*}
    
  
  \subsection*{$\int{x\sin{x}\cos{x}\ dx}$}
  \begin{align*}
      &&&(\text{slow method})\\
      &&&= \cos(-x\cos{x} + \int{\cos{x}\ dx}) - \\
      &&&\hspace{100pt}\int{-\sin{x}(-x\cos{x} + \int{\cos{x}\ dx})}\ dx + c \\
      &&&= \cos(-x\cos{x} + \sin{x}) - \int{-\sin{x}(-x\cos{x} + \sin{x})}\ dx + c &\\
      &&&= -x\cos^2{x} + \sin{x}\cos{x} - \int{x\sin{x}\cos{x}}\ dx + \int{\sin^2{x}}\ dx + c &\\
      &&&= \sin{x}\cos{x} - x\cos^2{x} + \frac{1}{2}\int{1 - \cos{2x}}\ dx -\\ &&&\hspace{180pt}\int{x\sin{x}\cos{x}}\ dx + c &\\
      &&&= \sin{x}\cos{x} - x\cos^2{x} + \frac{1}{2}(x - \frac{1}{2}\sin{2x}) - \int{x\sin{x}\cos{x}}\ dx + c &\\
      &\iff \int{x\sin{x}\cos{x}\ dx} &&= \frac{1}{2}\sin{x}\cos{x} - \frac{1}{2}x\cos^2{x} + \frac{1}{4}x - \frac{1}{8}\sin{2x}
  \end{align*}
  
  \begin{align*}
      &&&(\text{fast method})\\
      &&&= \frac{1}{2}x\sin^2{x} - \frac{1}{2}\int{\sin^2{x}\ dx} + c \\[8pt]
      &&&= \frac{1}{2}x\sin^2{x} - \frac{1}{4}\int{1 - \cos{2x}\ dx} + c\\[8pt]
      &&&= \frac{1}{2}x\sin^2{x} - \frac{1}{4}\left(x - \frac{1}{2}\sin{2x}\right) + c \\[8pt]
      &&&= \frac{1}{2}x\sin^2{x} - \frac{1}{4}x + \frac{1}{8}\sin{2x} + c \\[8pt]
  \end{align*}
  
  \begin{align*}
      &&&(\text{alternative fast method})\\
      &&&= \int{x\left(\frac{1}{2}\sin{2x}\right)\ dx} \\[8pt]
      &&&= -\frac{1}{4}x\cos{2x} + \frac{1}{4}\int{\cos{2x}\ dx} + c\\
      &&&= -\frac{1}{4}x\cos{2x} + \frac{1}{8}\sin{2x} + c\\
      &&&= -\frac{1}{4}x(1 - 2\sin^2{x}) + \frac{1}{8}\sin{2x} + c\\
  \end{align*}
  
  
  \subsection*{$\int{\frac{\ln{x}}{x^5}\ dx}$:}
  \begin{align*}
      \text{Note: we know how to }&\text{differentiate }\ln{x}\\
      \text{but not how to }&\text{integrate it}\implies\text{integration by parts} \\
      &= -\frac{1}{4}x^{-4}\ln{x} + \frac{1}{4}\int{x^{-5}\ dx} + c \\[8pt]
      &= -\frac{1}{4}x^{-4}\ln{x} + -\frac{1}{16}x^{-4} + c \\[8pt]
  \end{align*}
  
  \subsection*{$\int{\arcsin{3x}\ dx}$:}
  \begin{align*}
    &= \int{(1)(\arcsin{3x})} \\[8pt]
    &= x\arcsin{3x} - \int{\frac{3x}{\sqrt{1 - 9x^2}}}\ dx \\[8pt]
    &= x\arcsin{3x} + \frac{1}{6}\int{\frac{1}{\sqrt{u}}}\ du &(u = 1 - 9x^2,\ du = -18x\ dx) \\[8pt]
    &= x\arcsin{3x} + \frac{1}{6}(2\sqrt{u}) + c \\[8pt]
    &= x\arcsin{3x} + \frac{1}{3}\sqrt{1 - 9x^2} + c \\[8pt]
  \end{align*}


\bigskip
\bigskip
\bigskip
\bigskip


\section*{Exponentials}
\bigskip

  \subsection*{$\int_0^1{\frac{3^x + 4^x}{5^x}}dx$:}
  \begin{align*}
      &= \int_0^1{{\left(\frac{3}{5}\right)}^x}dx +         \int_0^1{{\left(\frac{4}{5}\right)}^x}dx && \\[8pt]
      &= \frac{{\left(\frac{3}{5}\right)}^x}{\ln(\frac{3}{5})} + \frac{{\left(\frac{4}{5}\right)}^x}{\ln(\frac{4}{5})} \\[8pt]
      &= \frac{\frac{3}{5} - 1}{\ln(\frac{3}{5})} +
      \frac{\frac{4}{5} - 1}{\ln(\frac{4}{5})} \\[8pt]
      &= \frac{\frac{-2}{5}}{\ln(\frac{3}{5})} +
      \frac{\frac{-1}{5}}{\ln(\frac{4}{5})}
  \end{align*}
  
  \subsection*{$\int{30e^{-3x}{\left(1 + 3e^{-x}\right)}^5}\ dx$:}
  \begin{align*}
      &= \int{10e^{-2x}{\left(1 + 3e^{-x}\right)^5}(3e^{-x})}\ dx && \\[8pt]
      &= -10\int{\left(\frac{u - 1}{3}\right)^2{u^5}}\ du && \left(u = 1 + 3e^{-x} \iff e^{-x} = \frac{u - 1}{3};\ du = -3e^{-x}\right) \\[8pt]
      &= -10/9\int{\left(u^2 - 2u + 1\right){u^5}}\ du && \\[8pt]
      &= -10/9\int{\left(u^7 - 2u^6 + u^5\right)}\ du && \\[8pt]
      &= -10/9\left(\frac{u^8}{8} - \frac{2u^7}{7} + \frac{u^6}{6}\right) + c && \\[8pt]
      &= -10/9\biggl(\frac{(1 + 3e^{-x})^8}{8} - \frac{2(1 + 3e^{-x})^7}{7}&& + \frac{(1 + 3e^{-x})^6}{6}\biggr) + c
  \end{align*}


\bigskip
\bigskip
\bigskip
\bigskip



\section*{Trigonometric Functions}
\bigskip

  \subsection*{$\int{(2 + \tan{x})^2}\ dx$:}
   
  \begin{align*}
    &= \int{4 + 4\tan{x} + \tan^2{x}}\ dx && \\[8pt]
    &= \int{4 + 4\tan{x} + (\sec^2{x} - 1)}\ dx && \\[8pt]
    &= 4x + 4\ln{\lvert\sec{x}\rvert} + \tan{x} - x + c && \\[8pt]
    &= 3x + 4\ln{\lvert\sec{x}\rvert} + \tan{x} + c
  \end{align*}
  
  
  \subsection*{$\int{\sin^3{x}}\ dx$:}
   
  \begin{align*}
    &= \int{(1 - \cos^2{x})\sin{x}}\ dx && \\[8pt]
    &= -\int{1 - u^2}\ du && (u = \cos{x},\ du = -\sin{x}\ dx)  \\[8pt]
    &= \frac{u^3}{3} - u + c && \\[8pt]
    &= \frac{\cos^3{x}}{3} - \cos{x} + c
  \end{align*}
  
  
  \subsection*{$\int{\frac{\cos^2{x}}{1 + \sin{x}}}\ dx$:}
   
  \begin{align*}
    &= \int{\frac{1 - \sin^2{x}}{1 + \sin{x}}}\ dx && \\[8pt]
    &= \int{\frac{(1 + \sin{x})(1 - \sin{x})}{1 + \sin{x}}}\ dx && \\[8pt]
    &= \int{1 - \sin{x}}\ dx && \\[8pt]
    &= x + \cos{x} + c
  \end{align*}
  
  
  \subsection*{$\int{\frac{\sin{x}}{1 + \sin{x}}}\ dx$:}
   
  \begin{align*}
    &= \int{\frac{\sin{x}(1 - \sin{x})}{(1 + \sin{x})(1 - \sin{x})}}\ dx && \\[8pt]
    &= \int{\frac{\sin{x} - \sin^2{x}}{1 - \sin^2{x}}}\ dx && \\[8pt]
    &= \int{\frac{\sin{x}}{\cos^2{x}}}\ dx - \int{\tan^2{x}}\ dx && \\[8pt]
    &= \int{\sec{x}\tan{x}}\ dx - \int{\sec^2{x} - 1}\ dx && \\[8pt]
    &= \sec{x} - \tan{x} - x + c
  \end{align*}
  
  
  \subsection*{$\int{(\csc{3x} + \cot{3x})^2}\ dx$:}
   
  \begin{align*}
    &= \int{\csc^2{3x} + 2\csc{3x}\cot{3x} + \cot^2{3x}}\ dx && \\[8pt]
    &= \int{\csc^2{3x}} + 2\int{\csc{3x}\cot{3x}} + \int{\csc^2{3x} - 1}\ dx && \\[8pt]
    &= 2\int{\csc^2{3x}} + 2\int{\csc{3x}\cot{3x}} - \int{1}\ dx && \\[8pt]
    &= 2(-\frac{\cot{3x}}{3})) + 2(-\frac{\csc{3x}}{3})) - x + c\ dx && \\[8pt]
    &= \frac{-2}{3}(\csc{3x} + \cot{3x}) - x + c
  \end{align*}
  
  
  \subsection*{$\int{\tan^5{x}}\ dx$:}
   
  \begin{align*}
    &= \int{\tan^3{x}(\sec^2{x} - 1)}\ dx && \\[8pt]
    &= \int{\tan^3{x}\sec^2{x}}\ dx - \int{\tan^3{x}}\ dx && \\[8pt]
    &= \int{\tan^3{x}\sec^2{x}}\ dx - \int{\tan{x}(\sec^2 - 1)}\ dx && \\[8pt]
    &= \int{\tan^3{x}\sec^2{x}}\ dx - \int{\tan{x}\sec^2}\ dx - \int{\tan{x}}\ dx && \\[8pt]
    &= \frac{1}{4}\tan^4{x} - \frac{1}{2}\tan^2{x} - \ln{\lvert\sec{x}\rvert} + c
  \end{align*}
  
  
  \subsection*{$\int{\sec{x}\sqrt{\sec{x} + \tan{x}}}\ dx$:}
   
  \begin{align*}
    &= \int{\frac{\sec{x}\sqrt{\sec{x} + \tan{x}}}{\sec{x}(\sec{x} + \tan{x})}}\ dx && (u = \sec{x} + \tan{x},\ du = \sec{x}\tan{x} + \sec^2{x})  \\[8pt]
    &= \int{\frac{\sqrt{u}}{u}}\ du \\[8pt]
    &= \int{\frac{1}{\sqrt{u}}}\ du \\[8pt]
    &= 2u^{\frac{1}{2}} + c \\[8pt]
    &= 2\sqrt{\sec{x} + \tan{x}} + c
  \end{align*}
  
  
  \subsection*{$\int{\frac{\sin{2x} - \cos{2x}}{\sin{2x} + \cos{2x}}}\ dx$:}
   
  \begin{align*}
    &\text{wrong way:} \\
    &= \int{\frac{ (\sin{2x} - \cos{2x})(\sin{2x} + \cos{2x}) }{ (\sin{2x} + \cos{2x})^2 }\ dx} \\
    &= \int{\frac{ \sin^2{2x} - \cos^2{2x} }{ 2\sin{2x}\cos{2x} }\ dx} &&\left(=\int{\frac{f(x)}{\frac{1}{2}f'(x)}\ dx}\right)\ \wrong \\
    &\text{another wrong way:} \\
    &= \frac{1}{2}\int{u\frac{dx}{du}\ dx}\ \wrong &&(u = \sin{2x} - \cos{2x}) \\[8pt]
    &\text{right way:} \\
    &= -\frac{1}{2}\int{\frac{1}{u}\frac{du}{dx}\ dx} &&(u = \sin{2x} + \cos{2x}) \\[8pt]
    &= -\frac{1}{2}\int{\frac{1}{u}\frac{du}{dx}\ dx} &&(u = \sin{2x} + \cos{2x}) \\[8pt]
    &= -\frac{1}{2}\int{\frac{1}{u}du\ dx} &&(u = \sin{2x} + \cos{2x}) \\[8pt]
    &= -\frac{1}{2}\ln{\rvert{u}\lvert} + c \\[8pt]
    &= -\frac{1}{2}\ln{\rvert{\sin{2x} + \cos{2x}}\lvert} + c \\
  \end{align*}

\bigskip
\bigskip
\bigskip
\bigskip

\section*{Trig-substitution}
\bigskip

  \subsection*{$\int_1^b{\frac{\sqrt{x^2 + 1}}{x}}dx$:}
   
  \begin{align*}
      & \int_1^b{\frac{\sqrt{x^2 + 1}}{x}}dx && \\[8pt]
      &= \int_1^b{\frac{\sqrt{\tan^2{\theta} + 1}}{\tan{\theta}}}\ d\tan{\theta} && \\[8pt]
      &= \int_{\arctan{1}}^{\arctan{b}}{\frac{\sec^3{\theta}}{\tan{\theta}}}\ d{\theta} && \\[8pt]
      &= \int_{\arctan{1}}^{\arctan{b}} {
          \frac{\sec{\theta}}{\tan{\theta}}(1 + \tan^2{\theta})
        }\ d{\theta} \\[8pt]
      &= \int_{\arctan{1}}^{\arctan{b}} { 
          \frac{\sec{\theta}}{\tan{\theta}} 
        }\ d{\theta} + \left[\sec{\theta}\right]_{\arctan{1}}^{\arctan{b}} \\[8pt]
      &= \int_{\arctan{1}}^{\arctan{b}} { 
          \frac{\sec{\theta}}{\tan{\theta}} 
        }\ d{\theta} + (\sqrt{b^2+1} - \sqrt{2}) && (wrt.\ \theta: opp=b, adj=1, hyp=\sqrt{b^2+1}) \\[8pt]
      &= \int_{\arctan{1}}^{\arctan{b}} { 
          \csc{\theta} 
        }\ d{\theta} + (\sqrt{b^2+1} - \sqrt{2}) \\[8pt]
      &= \left[-\ln\lvert\csc{\theta} +\cot{\theta}\rvert\right]_{\arctan{1}}^{\arctan{b}} + \sqrt{b^2+1} - \sqrt{2} \\[10pt]
      &= \left[
          \left(-\ln\left\lvert \frac{\sqrt{b^2+1}}{b} + \frac{1}{b} \right\rvert\right) - 
          \left(-\ln\left\lvert \sqrt{2} + 1 \right\rvert\right)
         \right] \\[6pt]
         &\ \ \ \ \ \ \ \ + \sqrt{b^2+1} - \sqrt{2} \\[10pt]
      &= \ln\left\lvert{b} \right\rvert - \ln\left\lvert{\sqrt{b^2+1} + 1} \right\rvert + \ln\left\lvert \sqrt{2} + 1 \right\rvert \\[4pt]
         &\ \ \ \ \ \ \ \  + \sqrt{b^2+1} - \sqrt{2}
  \end{align*}
  
  
\end{document}
